Towards DVE.

IL/SimApx.v
@@ -1,5 +1,5 @@
 Require Import List Infra.Relations.
-Require Export Util Var Val Exp Env Map CSet AutoIndTac IL Sim.
+Require Export Util Var Val Exp Env Map CSet AutoIndTac IL Sim AllInRel.
 
 Set Implicit Arguments.
 Unset Printing Records.
@@ -96,12 +96,17 @@ Qed.
 Lemma simapx_coterminatesWith {S} `{StateType S} {S'} `{StateType S'} (σ1:S) (σ2:S')
 : simapx σ1 σ2 -> forall v, terminatesWith σ1 (Some v) -> terminatesWith σ2 (Some v).
 Proof.
-  intros. general induction H2. rewrite Heqo.
-  + inv H3. exfalso. eapply H1. destruct H0; firstorder. 
-    destruct H4. eapply terminatesWith_star; eauto. econstructor; eauto.
-    congruence. admit. admit.
+  intros. remember (Some v). revert Heqo. induction H2; intros.
+  + inv H1.
+    - exfalso. eapply H3. destruct H4; firstorder. 
+    - destruct H5. 
+      * eapply terminatesWith_star; eauto. rewrite H4. econstructor; eauto.
+      * exfalso. firstorder.
+    - destruct H5. 
+      * congruence.
+      * exfalso. firstorder.
   + eapply IHterminatesWith. 
-    pose proof (simapx_step_closed _ H3 H0). eauto. reflexivity.
+    pose proof (simapx_step_closed _ H1 H2); eauto. eauto.
 Qed.
 
 Lemma coterminatesWith_simapx {S} `{StateType S} {S'} `{StateType S'} (σ1:S) (σ2:S') v
@@ -113,7 +118,7 @@ Proof.
   destruct H1, H2; dcr.
   eapply simE; eauto using star. rewrite H6, H8; reflexivity.
 Qed.
-(*
+
 Lemma sim_apxbehave {S} `{StateType S} {S'} `{StateType S'} (σ1:S) (σ2:S')
 : simapx σ1 σ2 <-> apxbehave σ1 σ2.
 Proof.
@@ -124,41 +129,270 @@ Proof.
     destruct (step_dec σ1) as [[]|]; destruct (step_dec σ2) as [[]|].
     - eapply simS; try eapply plusO; try eassumption. 
       eapply sim_apxbehave. eapply apxbehave_reduction_closed; eauto using star.
-    - pose proof (normal_terminates H3).
-      eapply terminatesWith_terminates in H4; destruct H4. 
-      destruct x0.
-      assert (terminatesWith σ1 (Some v)). eapply H1; eauto.
-      eapply coterminatesWith_sim; eauto.
-    - pose proof (normal_terminates H2). eapply terminatesWith_terminates in H4; destruct H4.
-      assert (terminatesWith σ2 x0). eapply H1; eauto.
-      eapply coterminatesWith_sim; eauto.
-    - pose proof (normal_terminates H2). eapply terminatesWith_terminates in H4; destruct H4.
-      assert (terminatesWith σ2 x). eapply H1; eauto.
-      eapply coterminatesWith_sim; eauto.
-Qed.
+    - exfalso; clear_all; admit. 
+    - exfalso; clear_all; admit.
+    - case_eq (result σ1); intros.
+      destruct H1; exploit H5. econstructor; eauto.
+      eapply simE; try eapply star_refl; eauto.
+      inv X. congruence. exfalso; firstorder. 
+      eapply simErr; eauto using star_refl.
+Admitted.
 
-Lemma cobehave_trans {S} `{StateType S} {S'} `{StateType S'} {S''} `{StateType S''} 
+Lemma apxbehave_trans {S} `{StateType S} {S'} `{StateType S'} {S''} `{StateType S''} 
 (σ1:S) (σ2:S') (σ3:S'')
-: cobehave σ1 σ2 -> cobehave σ2 σ3 -> cobehave σ1 σ3.
+: apxbehave σ1 σ2 -> apxbehave σ2 σ3 -> apxbehave σ1 σ3.
 Proof. 
   unfold cobehave; intros. destruct H2, H3; firstorder.
 Qed.
 
-Lemma sim_trans {S1} `{StateType S1} {S2} `{StateType S2} {S3} `{StateType S3}
-      (σ1:S1) (σ2:S2) (σ3:S3)
-  : sim σ1 σ2 -> sim σ2 σ3 -> sim σ1 σ3.
+Lemma simapx_trans {S1} `{StateType S1} 
+      (σ1:S1) {S2} `{StateType S2} (σ2:S2) {S3} `{StateType S3} (σ3:S3)
+  : simapx σ1 σ2 -> simapx σ2 σ3 -> simapx σ1 σ3.
 Proof.
   intros. 
-  rewrite sim_cobehave in H2. 
-  rewrite sim_cobehave in H3. 
-  rewrite sim_cobehave. 
-  pose proof (cobehave_trans H2 H3); eauto.
+  rewrite sim_apxbehave in H2. 
+  rewrite sim_apxbehave in H3. 
+  rewrite sim_apxbehave. 
+  pose proof (apxbehave_trans H2 H3); eauto.
+Qed.
+
+Lemma simapx_expansion_closed {S} `{StateType S} 
+      (σ1 σ1':S) {S'} `{StateType S'} (σ2 σ2':S')
+  : simapx σ1' σ2'
+    -> star step σ1 σ1' 
+    -> star step σ2 σ2'
+    -> simapx σ1 σ2.
+Proof.
+Admitted.
+
+Definition ParamRel A := A-> list var -> list var -> Prop.
+Definition ArgRel A := A-> list val -> list val -> Prop.
+
+Inductive simB {A} (R:ArgRel A) (R':ParamRel A) : F.labenv -> F.labenv -> A -> F.block -> F.block -> Prop :=
+| simBI a L L' E E' Z Z' s s'
+  : R' a Z Z'
+    -> (forall VL VL', R a VL VL' -> length Z = length VL -> length Z' = length VL'
+                 -> simapx (L, E[Z <-- VL], s) 
+                          (L', E'[Z' <-- VL'], s'))
+    -> simB R R' L L' a (F.blockI E Z s) (F.blockI E' Z' s').
+
+Definition simL {A} R R' (AL:list A) L L' := AIR5 (simB R R') L L' AL L L'.
+(*
+Lemma simL_refl {A} R (AL:list A) L : 
+  length AL = length L -> simL R AL L L.
+Proof.
+  general induction L. destruct AL; isabsurd. constructor.
+  destruct AL; isabsurd.
+  econstructor; eauto. destruct a; econstructor; eauto. intros. eapply sim_refl.
+  eapply IHL. simpl in *; omega.
+Qed.
+
+Lemma simL_sym L1 L2 L3 L4 : AIR4 simB L1 L2 L3 L4 -> AIR4 simB L2 L1 L4 L3.
+Proof.
+  intros. general induction H; eauto using AIR4.
+  econstructor; eauto.
+  destruct pf. 
+  econstructor; eauto. intros. refine (sim_sym _). eapply H1; eauto. congruence. 
+Qed.
+
+Lemma simL_trans LA1 LA2 LB1 LB2 LC1 LC2 
+ : AIR4 simB LA1 LB1 LA2 LB2 -> AIR4 simB LB1 LC1 LB2 LC2
+-> AIR4 simB LA1 LC1 LA2 LC2.
+Proof.
+  intros. general induction H; inv H0; eauto using AIR4.
+  econstructor; eauto. inv pf. inv pf0.
+  econstructor. congruence.
+  intros. refine (sim_trans (H2 _ _ _) (H11 _ _ _)); congruence.
 Qed.
 *)
 
+Definition simeq2 {A} R R' (AL:list A) (s s':stmt)
+  := forall (L L':F.labenv) E, simL R R' AL L L' -> sim (L, E, s) (L', E, s').
+
+Definition fexteq {A} (R:ArgRel A) R' (a:A) (AL:list A) E Z s E' Z' s' := 
+  forall VL VL' L L', R a VL VL' -> simL R R' AL L L' 
+                 -> length Z = length VL
+                 -> length Z' = length VL'
+                 -> simapx (L, E[Z <-- VL], s) 
+                       (L', E'[Z' <-- VL'], s').
+(*
+Lemma fexteq_sym E Z s E' Z' s' 
+: fexteq E Z s E' Z' s' <-> fexteq E' Z' s' E Z s.
+Proof.
+  unfold fexteq; intuition.
+  - eapply sim_sym, H, simL_sym; eauto; congruence.
+  - eapply sim_sym, H, simL_sym; eauto; congruence.
+Qed.
+*)
+(*
+Lemma subst_lemma_div_L L L1 L2 s s' E E1 E2 Z Z' t
+: fexteq E1 Z s E2 Z' s'
+  -> length Z = length Z'
+  -> simL L1 L2
+  -> diverges step ((L ++ F.blockI E1 Z s :: L1)%list, E, t)
+  -> diverges step ((L ++ F.blockI E2 Z' s' :: L2)%list, E, t).
+Proof.
+  revert L L1 L2 s s' E E1 E2 Z Z' t. cofix; intros.
+  inv H2; inv H3.
+  + econstructor. constructor; eauto. eauto.
+  + econstructor. econstructor; eauto. eauto.
+  + econstructor. eapply F.stepIfF; eauto. eauto. 
+  + destruct (get_subst _ _ _ Ldef) as [?|[?|?]]; subst; simpl in *; dcr.
+    - econstructor. econstructor. eapply len. eapply get_app; eauto. reflexivity.
+      pose proof (get_range H5). rewrite drop_length; eauto.
+      rewrite drop_length in H4; eauto.
+    - subst; simpl in *. 
+      econstructor. constructor. instantiate (1:= F.blockI E2 Z' s').
+      simpl. congruence. simpl. rewrite H7. eapply get_length_app.
+      reflexivity. simpl. rewrite H7. rewrite drop_length_eq.
+      eapply (subst_lemma_div_L nil); eauto. simpl. 
+      rewrite H7 in H4. rewrite drop_length_eq in H4. unfold updE.
+      specialize (H (lookup_list E Y)).
+      pose proof (@sim_codiverge F.state _ F.state _).
+      eapply H5; eauto. eapply H. 
+      rewrite lookup_list_length. congruence. congruence.
+      eapply simL_refl.
+    - edestruct (AIR4_length H1); dcr.
+      destruct (AIR4_nth' H1 H6) as [? [? [?]]]; dcr.
+      inv H15. repeat (get_functional; subst). simpl in *.
+      econstructor. econstructor. Focus 2.
+      rewrite cons_app. rewrite app_assoc. 
+      eapply get_app_right; eauto. simpl.
+      repeat rewrite app_length; simpl. omega. simpl. congruence.
+      reflexivity. simpl. rewrite drop_length_gr; eauto.
+      rewrite drop_length_gr in H4; eauto.
+      pose proof (@sim_codiverge F.state _ F.state _).
+      eapply H6. eapply H14. rewrite lookup_list_length. congruence. congruence.
+      eauto. 
+  + econstructor. econstructor.
+    rewrite cons_app. rewrite app_assoc.
+    eapply (subst_lemma_div_L (F.blockI E Z0 s0::nil ++ L)%list); eauto.
+Qed.
+
+Lemma subst_lemma_trm_L L L1 L2 s s' E E1 E2 Z Z' t v
+: fexteq E1 Z s E2 Z' s'
+  -> length Z = length Z'
+  -> simL L1 L2
+  -> terminatesWith ((L ++ F.blockI E1 Z s :: L1)%list, E, t) v
+  -> terminatesWith ((L ++ F.blockI E2 Z' s' :: L2)%list, E, t) v.
+Proof.
+  intros LEQ H LEN H0.
+  general induction H0.
+  + constructor. eauto. hnf; intros. eapply H0.
+    destruct H; inv H.
+    - eexists; econstructor; eauto.
+    - eexists; econstructor; eauto.
+    - eexists; eapply F.stepIfF; eauto.
+    - edestruct (get_subst) as [|[]]; eauto.
+      * econstructor; econstructor; eauto. eapply get_app; eauto.
+      * dcr; subst. 
+        econstructor. econstructor; try (rewrite H4; eapply get_length_app); eauto.
+        simpl in * |- *; congruence.
+      * dcr; subst.
+        edestruct AIR4_length; try eassumption; dcr.
+        edestruct (get_length_eq _ H3 (eq_sym H2)); eauto.
+        unfold simL in *. edestruct AIR4_nth as [blk1 [blk2]]; eauto; dcr.
+        inv H12; repeat get_functional; subst.
+        econstructor; econstructor.
+        Focus 2.
+        eapply get_app_right. instantiate (1:=S (counted l - S (length L))).
+        omega. econstructor; eauto. simpl in * |- *; congruence.
+        reflexivity.
+    - econstructor; econstructor; eauto. 
+  + inv H.
+    - eapply trmWithStep. econstructor; eauto.
+      eapply IHterminatesWith; eauto.
+    - eapply trmWithStep. econstructor; eauto.
+      eapply IHterminatesWith; eauto.
+    - eapply trmWithStep. eapply F.stepIfF; eauto.
+      eapply IHterminatesWith; eauto.
+    - destruct (get_subst _ _ _ Ldef) as [|[|]].
+      * eapply trmWithStep. econstructor. eapply len.
+        eapply get_app; eauto. reflexivity.
+        rewrite drop_length; eauto using get_range.
+        eapply IHterminatesWith; eauto.
+        rewrite drop_length; eauto using get_range.
+      * dcr; subst.
+        edestruct AIR4_length; eauto; dcr.
+        eapply trmWithStep. econstructor.
+        Focus 2.
+        rewrite H4. eapply get_length_app. 
+        simpl in * |- *. congruence. reflexivity.
+        simpl.
+        rewrite H4 in *. erewrite drop_length_eq in *. 
+        simpl in *. rewrite H4. erewrite drop_length_eq. 
+        unfold updE.
+        refine (sim_coterminatesWith (LEQ (lookup_list E Y) _ _ 
+                                               _ _ (simL_refl _)) _).
+        rewrite lookup_list_length. congruence. congruence.
+        eapply (IHterminatesWith nil); eauto. 
+      * dcr.
+        edestruct AIR4_length; try eassumption; dcr.
+        edestruct get_length_eq; try eassumption.
+        edestruct AIR4_nth as [blk1 [blk2]]; dcr; eauto.
+        inv H12; repeat get_functional; subst. simpl in *.
+        eapply trmWithStep. econstructor.
+        Focus 2.
+        rewrite cons_app; rewrite app_assoc.
+        eapply get_app_right; eauto. rewrite app_length; simpl in *. omega.
+        simpl in * |- *; congruence. reflexivity.
+        rewrite drop_length_gr; eauto.
+        rewrite drop_length_gr in H0; eauto.
+        unfold updE.
+        simpl. 
+        refine (sim_coterminatesWith (H10 _ _ _) _). 
+        rewrite lookup_list_length. simpl in *. congruence. congruence.
+        eapply H0.
+    - eapply trmWithStep. econstructor; eauto.
+      rewrite cons_app. rewrite app_assoc.
+      eapply IHterminatesWith; eauto.
+Qed.
+*)
+
+(*
+Lemma subst_lemma_L A R (a:A) AL s s' V E E' Z Z' L1 L2 t
+: fexteq R a AL E Z s E' Z' s'
+  -> length Z = length Z'
+  -> simL R AL L1 L2
+  -> sim (F.blockI E Z s :: L1, V, t)
+         (F.blockI E' Z' s' :: L2, V, t').
+Admitted.
+*)
+
+Lemma subst_lemma A R R' (a:A) AL s s' V V' E E' Z Z' L1 L2 t t'
+: fexteq R R' a (a::AL) E Z s E' Z' s'
+  -> R' a Z Z'
+  -> simL R R' AL L1 L2
+  -> (forall (L L' : list F.block),
+       simL R R' (a :: AL) L L' ->
+       simapx (L, V, t) (L', V', t'))
+  -> simapx (F.blockI E Z s :: L1, V, t)
+         (F.blockI E' Z' s' :: L2, V', t').
+Proof.
+  revert_all; cofix; intros.
+  eapply H2. econstructor; eauto.
+  constructor; try eassumption. intros.
+  eapply H; try eassumption.
+Admitted.
+
+
+
+Lemma simL_extension A R R' (a:A) AL s s' E E' Z Z' L L'
+: simL R R' AL L L' 
+  -> fexteq R R' a (a::AL) E Z s E' Z' s'
+  -> R' a Z Z'
+  -> simL R R' (a::AL) (F.blockI E Z s :: L) (F.blockI E' Z' s' :: L').
+Proof.
+  intros.
+  hnf; intros. econstructor; eauto. econstructor; eauto; intros.
+  + hnf in H0.
+    eapply subst_lemma; eauto. 
+Qed.
+
+
 (* 
 *** Local Variables: ***
-*** coq-load-path: (("../" "Lyn")) ***
+*** coq-load-path: (("../" "Lvc")) ***
 *** End: ***
 *)
 
