DeadVariableElimination.v
@@ -1,0 +1,621 @@
+Require Import CSet Le.
+
+Require Import Plus Util AllInRel Map.
+Require Import Val Var Env EnvTy IL ParamsMatch Sim SimApx Alpha Coherence Fresh.
+
+Require Import Liveness.
+
+Set Implicit Arguments.
+Unset Printing Records.
+
+Opaque compute_prop.
+
+Notation "B[ x ]" := (if [ x ] then true else false).
+
+Fixpoint filter_by {A B} (f:A -> bool) (L:list A) (L':list B) : list B :=
+  match L, L' with
+    | x :: L, y::L' => if f x then y :: filter_by f L L' else filter_by f L L' 
+    | _, _ => nil
+  end.
+
+Fixpoint compile (s:stmt) (a:ann live) :=
+  match s, a with
+    | stmtExp x e s, annExp lv an => 
+      if [x ∈ getAnn an] then stmtExp x e (compile s an)
+                         else compile s an
+    | stmtIf x s t, annIf _ ans ant => stmtIf x (compile s ans) (compile t ant)
+    | stmtGoto f Y, annGoto lv => 
+      stmtGoto f (List.filter (fun y => B[y ∈ lv]) Y) 
+    | stmtReturn x, annReturn _ => stmtReturn x
+    | stmtLet Z s t, annLet lv ans ant => 
+      stmtLet (List.filter (fun x => B[x ∈ getAnn ans]) Z)
+              (compile s ans) (compile t ant)
+    | s, _ => s
+  end.
+
+Definition ArgRel (G:(live * params)) (VL VL': list val) : Prop := 
+  VL' = (filter_by (fun x => B[x ∈ (fst G)]) (snd G) VL).
+
+Definition ParamRel (G:(live * params)) (Z Z' : list var) : Prop := 
+  Z' = (List.filter (fun x => B[x ∈ (fst G)]) Z) /\ snd G = Z.
+
+Lemma lookup_list_filter_by_commute A B C (V:A->B) (Z:list C) Y p
+: length Z = length Y 
+  -> lookup_list V (filter_by p Z Y) =
+    filter_by p Z (lookup_list V Y).
+Proof.
+  intros. eapply length_length_eq in H. 
+  general induction H; simpl; eauto.
+  + destruct if; simpl; rewrite IHlength_eq; eauto.
+Qed.
+
+Lemma argsLive_filter_length lv blv Z Y
+: argsLive lv blv Y Z
+  -> length (List.filter (fun x : var => B[x ∈ blv]) Z) =
+    length (List.filter (fun y : var => B[y ∈ lv]) Y).
+Proof.
+  intros. general induction H; simpl; eauto.
+  destruct_prop (z ∈ blv); destruct_prop (y ∈ lv); try tauto; simpl.
+  - rewrite IHargsLive; eauto.
+Qed.
+
+Lemma filter_incl lv Y
+  : of_list (List.filter (fun y : var => B[y ∈ lv]) Y) ⊆ lv.
+Proof.
+  general induction Y; simpl. 
+  - cset_tac; intuition.
+  - destruct_prop (a ∈ lv); simpl. cset_tac; intuition. rewrite <- H0; eauto.
+    rewrite <- IHY; eauto.
+    eauto.
+Qed.
+
+Tactic Notation "destruct-if" "in" hyp(H) :=
+  match goal with 
+    | H : context [if sumbool_bool ?P then _ else _] |- _ => destruct P
+    | H : context [if ?P then _ else _] |- _ => destruct P
+  end.
+
+Tactic Notation "destruct-if" :=
+  match goal with
+    | |- context [if (if ?P then true else false) then _ else _] => destruct P
+    | |- context [if ?P then _ else _] => destruct P
+  end.
+
+Lemma argsLive_filter_filter_by lv blv Y Z
+: argsLive lv blv Y Z
+  -> List.filter (fun y : var => B[y ∈ lv]) Y
+    = filter_by (fun x : var => B[x ∈ blv]) Z Y.
+Proof.
+  intros. general induction H; simpl; eauto.
+  repeat destruct-if; try tauto.
+  rewrite IHargsLive; eauto.
+Qed.
+
+Lemma agree_on_update_filter lv (V:var -> val) Z VL 
+: length Z = length VL
+  -> agree_on lv 
+             (V [Z <-- VL])
+             (V [List.filter (fun x => B[x ∈ lv]) Z <--
+                             filter_by (fun x => B[x ∈ lv]) Z VL]).
+Proof.
+  intros. eapply length_length_eq in H.
+  general induction H.
+  - eapply agree_on_refl.
+  - simpl. repeat destruct-if. simpl. eapply agree_on_update_same.
+    eapply agree_on_incl. eapply IHlength_eq. cset_tac; intuition.
+    eapply agree_on_update_dead; eauto.
+Qed.
+
+Lemma agree_on_update_filter' (lv:set var) (V V':var -> val) Z VL 
+: length Z = length VL
+  -> agree_on (lv \ of_list Z) V V'
+  -> agree_on lv 
+             (V [Z <-- VL])
+             (V' [List.filter (fun x => B[x ∈ lv]) Z <--
+                             filter_by (fun x => B[x ∈ lv]) Z VL]).
+Proof.
+  intros.
+  pose proof (update_with_list_agree _ VL H0 H).
+  eapply agree_on_trans. eapply H1.
+  eapply agree_on_update_filter. eauto.
+Qed.
+
+Definition blockRel (AL:list (live*params)) L (L':F.labenv) := (forall n blk lvZ, get AL n lvZ -> get L n blk -> block_Z blk = snd lvZ).
+           
+Lemma sim_DVE L L' V V' s LV lv
+: agree_on (getAnn lv) V V'
+-> true_live_sound LV s lv
+-> simL ArgRel ParamRel LV L L'
+-> @simapx F.state _ F.state _ (L,V, s) (L',V', compile s lv).
+Proof.
+  general induction s; simpl; inv H0; simpl in * |- *.
+  + case_eq (exp_eval V e); intros. destruct if. 
+    - eapply simS; try eapply plusO.
+      econstructor; eauto.
+      econstructor; eauto. instantiate (1:=v).
+      erewrite exp_eval_live; eauto using agree_on_sym.
+      eapply IHs; eauto. eapply agree_on_update_same. 
+      eapply agree_on_incl; eauto. 
+    - eapply simapx_expansion_closed; 
+      [ | eapply S_star; [ econstructor; eauto | eapply star_refl ]
+        | eapply star_refl].
+      eapply IHs; eauto. eapply agree_on_update_dead; eauto.
+      eapply agree_on_incl; eauto. rewrite <- H9. cset_tac; intuition.
+    - eapply simErr; [| eapply star_refl|]; eauto. stuck.
+  + case_eq (val2bool (V x)); intros.
+    eapply simS; try eapply plusO.
+    econstructor; eauto. econstructor; eauto. 
+    rewrite <- H; eauto. eapply IHs1; eauto using agree_on_incl.
+    eapply simS; try eapply plusO.
+    econstructor 3; eauto. econstructor 3; eauto.
+    rewrite <- H; eauto. eapply IHs2; eauto using agree_on_incl.
+  + destruct (get_dec L (counted l)) as [[[bE bZ bs]]|].
+(*    hnf in H2. exploit H2; eauto. simpl in *. subst bZ. *)
+    destruct_prop (length Z = length Y). 
+    unfold simL in H1.
+    edestruct AIR5_length; try eassumption; dcr.
+    edestruct get_length_eq; try eassumption.
+    edestruct AIR5_nth as [?[? [?]]]; try eassumption; dcr. 
+    simpl in *. repeat get_functional; subst.
+    inv H16. hnf in H20. dcr; simpl in *. subst bZ.
+    eapply simS; try eapply plusO.
+    econstructor; eauto. simpl. congruence.
+    econstructor; eauto. simpl. hnf in H21. dcr. simpl in *. subst.
+    simpl.  
+    eapply argsLive_filter_length; eauto.
+    simpl in * |- *.
+    unfold updE. eapply H21.
+    hnf. simpl. 
+    rewrite <- lookup_list_filter_by_commute.
+    exploit argsLive_filter_filter_by; eauto.
+    rewrite <- X. eapply lookup_list_agree.
+    eapply agree_on_incl; eauto using agree_on_sym.
+    eapply filter_incl; eauto.
+    congruence.
+    eapply simE; try eapply star_refl; eauto; stuck.
+    eapply simE; try eapply star_refl; eauto; stuck; eauto.
+    edestruct AIR5_length; try eassumption; dcr.
+    edestruct get_length_eq; try eassumption.
+    simpl in *. repeat get_functional; subst.
+    admit.
+  + eapply simE; try eapply star_refl.
+    simpl. rewrite H; eauto. simpl. 
+    stuck. stuck.
+  + econstructor; try eapply plusO.
+    econstructor; eauto.
+    econstructor; eauto.
+    simpl. eapply IHs2; eauto. 
+    - simpl in *; eapply agree_on_incl; eauto.
+    - eapply simL_extension; eauto. hnf; intros.
+      eapply IHs1; eauto.
+      * hnf in H2. subst. simpl.
+        eapply agree_on_update_filter'. eauto.
+        eapply agree_on_incl; eauto.
+      * split; reflexivity.
+Qed.
+
+(*
+
+Fixpoint natural {P} (f:P -> list var -> list var) (VL:list (option P)) (s:stmt) : stmt :=
+  match s with
+   | stmtExp x e s => stmtExp x e (natural f VL s)
+   | stmtIf x s1 s2 => stmtIf x (natural f VL s1) (natural f VL s2)
+   | stmtGoto l Y => match nth_error VL (counted l) with 
+                     | Some (Some p) => stmtGoto l (f p Y)
+                     | _ => stmtGoto l Y
+                     end
+   | stmtReturn x => stmtReturn x
+   | stmtLet Z s1 s2 => stmtLet Z (natural f (None::VL) s1) (natural f (None::VL) s2)
+   end.
+
+Inductive simB {P} (R: P -> list val -> list val -> Prop) 
+: P -> F.labenv -> F.labenv -> F.block -> F.block -> Prop :=
+| simBI p L L' E E' Z Z' s s'
+  : 
+    (forall VL VL', R p VL VL'  
+                       -> sim (L, E[Z <-- VL], s) 
+                              (L', E'[Z' <-- VL'], s'))
+    -> simB R p L L' (F.blockI E Z s) (F.blockI E' Z' s').
+
+Definition simL P (R: P -> list val -> list val -> Prop) PL L L' 
+  := AIR5 (simB R) PL L L' L L'.
+
+Definition comp {P} (R R':P -> list val -> list val -> Prop) p VL VL' :=
+  exists VL'', R p VL VL'' /\ R' p VL'' VL'.
+
+Definition compf {P} (f f':P -> list val -> list val) p VL :=
+  f' p (f p VL).
+
+Definition implements {P} (R:P -> list val -> list val -> Prop) (f:P -> list var -> list var)
+  := forall (p:P) (L:list var) E, R p (lookup_list E L) (lookup_list E (f p L)).
+
+Lemma subst_lemma_R P (R: P -> list val -> list val -> Prop) s s' V E E' Z Z' L1 L2 t p PL f
+: (forall L L', simL R PL L L' -> 
+       forall VL VL', R p VL VL' ->
+        sim (L, E[Z <-- VL], s) 
+            (L', E'[Z' <-- VL'], s'))
+  -> simL R PL L1 L2
+  -> implements R f
+  -> sim ((F.blockI E Z s :: L1)%list, V, t)
+         ((F.blockI E' Z' s' :: L2)%list, V, natural f (List.map Some (p::PL)) t).
+Proof.
+Admitted.
+
+Lemma R_intro P (R: P -> list val -> list val -> Prop) V L1 L2 t PL f
+: simL R PL L1 L2
+  -> implements R f
+  -> sim (L1, V, t)
+         (L2, V, natural f (List.map Some PL) t).
+Proof.
+Admitted.
+
+
+Lemma simL_split P (R R': P -> list val -> list val -> Prop) L1 L3 PLA
+ : simL (comp R R') PLA L1 L3 -> exists PLB PLC L2,
+simL R PLB L1 L2 /\ simL R' PLC L2 L3.
+Proof.
+  intros. hnf in H. induction H. do 3 eexists nil; split; econstructor.
+  edestruct IHAIR5 as [A [B []]]; dcr.
+  inv pf.
+  
+Qed.
+*)
+
+(*
+
+Lemma R_natural P (R R': P -> list val -> list val -> Prop) s s' E E' L1 L2 L3 PL PL' f'
+: (forall L L', simL R PL L L' -> 
+        sim (L, E, s) 
+            (L', E', s'))
+  -> simL R PL L1 L2
+  -> simL R' PL' L2 L3
+  -> implements R' f'
+  -> sim (L1, E, s)
+         (L3, E', natural f' (List.map Some PL') s').
+Proof.
+  intros. 
+  simpl.
+  refine (sim_trans (H _ _ _ ) _ ); try eassumption.
+  eapply R_intro; eauto.
+Qed.
+
+
+
+Lemma sim_shift P (R R': P -> list val -> list val -> Prop) s s' E E' L1 p PL f
+: implements R f
+  -> (forall L L', simL R  PL L L' ->
+       forall VL VL', R p VL VL' ->
+        sim (L, E, s)
+            (L', E', s'))
+  -> sim (L1, E, natural f (List.map Some (p::PL)) s)
+         (L1, E', s').
+Proof.
+  
+Admitted.
+
+
+Definition inv {P} (R: P -> list val -> list val -> Prop) p x y
+ := R p y x.
+
+Lemma simL_sym P (R: P -> list val -> list val -> Prop) PL L L'
+ : simL R PL L L' -> simL (inv R) PL L' L.
+Admitted.
+
+(*
+Lemma R_natural' P (R: P -> list val -> list val -> Prop) s s' E E' L PL f'
+: (forall L L', simL R PL L L' -> 
+        sim (L, E, s) 
+            (L', E', s'))
+  -> implements (inv R) f'
+  -> @sim F.state _ F.state _ (L, E, s)
+         (L, E', natural f' (List.map Some PL) s').
+Proof.
+  intros. 
+  simpl.
+  refine (sim_trans (H _ _ _ ) _); try eassumption.
+  eapply R_intro; eauto. eapply simL_sym; eauto.
+Qed.
+*)
+
+Lemma simL_extension' P (R: P -> list val -> list val -> Prop) (f: P -> list var -> list var) PL s s' E E' Z Z' L L' p
+: simL R PL L L' 
+  -> (forall L L', simL R PL L L' -> 
+                   forall VL VL', R p VL VL'  
+                                  -> sim (L, E[Z <-- VL], s) 
+                                         (L', E'[Z' <-- VL'], s'))
+  -> simL R (p::PL) (F.blockI E Z s :: L) (F.blockI E' Z' s' :: L').
+Proof.
+  intros.
+  hnf; intros. econstructor; eauto. econstructor; eauto; intros.
+
+  + refine (sim_trans (subst_lemma_R _ _ _  _ _ _ _ _ _ _ ) _); try eassumption.
+    instantiate (1:=f). admit.
+    eapply sim_sym.
+    eapply R_natural.
+    intros. eapply sim_sym. eapply H0; eauto.
+    eapply simL_sym; eauto.
+    instantiate (1:=(F.blockI E Z s::L)).
+    econstructor. econstructor.
+    instantiate (1:= inv R). admit. 
+    
+    
+    
+    
+    Focus 3.
+    instantiate (3:=E'). instantiate (2:=s'). instantiate (1:=L').
+    refine (sim_trans (H0 _ _ _ _ _ _) (sim_refl _)); try eassumption.
+    
+Admitted.
+
+
+Fixpoint compile (s:stmt) (a:ann live) :=
+  match s, a with
+    | stmtExp x e s, annExp lv an => 
+      if [x ∈ getAnn an] then stmtExp x e (compile s an)
+                         else compile s an
+    | stmtIf x s t, annIf _ ans ant => stmtIf x (compile s ans) (compile t ant)
+    | stmtGoto f Y, annGoto lv => 
+      stmtGoto f (List.filter (fun x => if [x ∈ lv] then true else false) Y)
+    | stmtReturn x, annReturn _ => stmtReturn x
+    | stmtLet Z s t, annLet lv ans ant => 
+      stmtLet (List.filter (fun x => if [x ∈ getAnn ans] then true else false) Z) 
+              (compile s ans) (compile t ant)
+    | s, _ => s
+  end.
+
+Lemma sim_DCE L L' V V' s G lv
+: agree_on (getAnn lv) V V'
+-> true_live_sound G s lv
+-> simL LiveRel G L L'
+-> @sim F.state _ F.state _ (L,V, s) (L',V', compile s lv).
+Proof.
+    general induction s; simpl; inv H0; simpl in * |- *.
+  + case_eq (exp_eval V e); intros. destruct if. 
+    - eapply simS; try eapply plusO.
+      econstructor; eauto.
+      econstructor; eauto. instantiate (1:=v). admit.
+      eapply IHs; eauto. eapply agree_on_update_same. 
+      eapply agree_on_incl; eauto. 
+    - eapply sim_expansion_closed.
+    Focus 2. eapply S_star. econstructor; eauto. 
+    eapply star_refl. Focus 2. eapply star_refl.
+    eapply IHs; eauto. eapply agree_on_update_dead; eauto.
+    eapply agree_on_incl; eauto. rewrite <- H9. cset_tac; intuition. 
+    - admit.
+  + admit.
+  + (* destruct (get_dec L (counted l)). destruct s as [[]].
+    destruct_prop (length block_Z = length Y). 
+    unfold simL in H1.
+    edestruct AIR5_length; try eassumption; dcr.
+    edestruct get_length_eq; try eassumption.
+    edestruct AIR4_nth as [?[?]]; try eassumption; dcr. 
+    simpl in *. repeat get_functional; subst.
+    inv H14. eapply simS; try eapply plusO.
+    econstructor; eauto. simpl. rewrite lookup_list_length. congruence.
+    econstructor; eauto. simpl. congruence.
+    simpl. unfold updE. assert (lookup_list V (lookup_list ϱ Y) = lookup_list V' Y).
+    rewrite <- comp_lookup_list. 
+    admit.
+    rewrite H5. eapply H19.
+    eapply simE; try eapply star_refl; eauto; stuck.
+    get_functional; subst. eapply n. simpl in *. rewrite len.
+    rewrite lookup_list_length; eauto.
+    edestruct AIR4_length; try eassumption; dcr.
+    edestruct get_length_eq; try eassumption.
+    edestruct AIR4_nth as [?[?]]; try eassumption; dcr. 
+    simpl in *. repeat get_functional; subst.
+    inv H14; simpl in *. eapply n. congruence.
+    eapply simE; try eapply star_refl; eauto; stuck; eauto.
+    edestruct AIR4_length; try eassumption; dcr.
+    edestruct get_length_eq; try eassumption. eauto. *)
+(*
+    admit.
+  + eapply simE; try eapply star_refl.
+    simpl. rewrite H; eauto. simpl. 
+    stuck. stuck.
+  + econstructor; try eapply plusO.
+    econstructor; eauto.
+    econstructor; eauto.
+    simpl. eapply IHs2; eauto. 
+    simpl in *; eapply agree_on_incl; eauto.
+    eapply simL_extension; eauto. intros.
+    eapply IHs1; eauto.
+    admit. admit.
+Qed.
+
+
+
+Fixpoint compile_spill (spill:list var) (cont:stmt) :=
+  match spill with
+  | nil => cont
+  | x::spill => stmtExp x (Var x) (compile_spill spill cont)
+  end.
+
+Fixpoint compile_reload (reload:list var) (cont:stmt) :=
+  match spill with
+  | nil => cont
+  | x::spill => stmtExp x (Var x) (compile_spill spill cont)
+  end.
+
+
+Fixpoint compile (s:stmt) (an:ann (list var*list var)) : stmt :=
+  match s, an with
+    | stmtExp x e s, annExp (spill,reload) an => 
+      compile_spill spill (compile_reload reload (stmtExp x e (compile s an)))
+    | stmtIf x s t, annIf (spill,reload) ans ant => 
+      compile_spill spill (compile_reload reload (stmtIf x (compile s ans) (compile t ant)))
+    | stmtGoto f Y, annGoto (spill,reload) => 
+      compile_spill spill (compile_reload reload (stmtGoto f (Y++Za)))
+    | stmtReturn x, annReturn (spill,reload) => 
+      compile_spill spill (compile_reload reload (stmtReturn x))
+    | stmtLet Z s t, annLet (spill, reload) ans ant =>
+      compile_spill spill (compile_reload reload (stmtLet (Z++Za) (compile s ans) (compile t ant)))
+    | s, _ => s
+  end.
+
+Lemma subst_alpha ϱ ϱ' s
+: inverse_on (freeVars s) ϱ ϱ'
+  -> alpha ϱ ϱ' s (substVars ϱ s).
+Proof.
+  general induction s; simpl in * |- *.
+  econstructor. admit.
+  eapply IHs. 
+  econstructor. eauto. admit.
+  eauto. eauto.
+  econstructor. eauto. admit.
+  econstructor. eauto. admit.
+  econstructor. eauto. eapply IHs1.
+  eapply IHs2.
+Qed.
+
+Fixpoint substVars (ϱ:var -> var) (s:stmt) : stmt :=
+  match s with
+   | stmtExp x e s => stmtExp x e (substVars (ϱ[x <- x]) s)
+   | stmtIf x s1 s2 => stmtIf (ϱ x) (substVars ϱ s1) (substVars ϱ s2)
+   | stmtGoto l Y => stmtGoto l (lookup_list ϱ Y)
+   | stmtReturn x => stmtReturn (ϱ x)
+   | stmtLet Z s1 s2 => stmtLet Z (substVars (ϱ[Z <-- Z]) s1) (substVars ϱ s2)
+   end.
+
+Lemma sim_eta L L' V V' s ϱ
+: (forall x, V' x = V (ϱ x))
+-> simL L L'
+-> @sim F.state _ F.state _ (L,V,substVars ϱ s) (L',V',s).
+Proof.
+Admitted.
+*)
+(*
+  revert_all. cofix; intros.
+  destruct s; simpl.
+  case_eq (exp_eval V e); intros.
+  eapply simS; try eapply plusO.
+  econstructor. eauto. 
+  econstructor. instantiate (1:=v). admit.
+  eapply sim_eta. admit.
+  admit.
+  case_eq (val2bool (V' x)); intros.
+  econstructor; try eapply plusO.
+  econstructor. rewrite <- H; eauto.
+  econstructor; eauto. admit.
+  econstructor; try eapply plusO.
+  eapply F.stepIfF. rewrite <- H. eauto.
+  eapply F.stepIfF. eauto.
+  admit.
+  admit.
+  admit.
+  econstructor; try eapply plusO.
+  econstructor. 
+  econstructor.
+Admitted.
+*)
+(*
+Lemma sim_spill L V V' ϱ (x y:var) s s'
+: s = substVars (ϱ[y <-ϱ x]) s'
+  -> (forall x, V' x = V (ϱ x))
+  -> @sim F.state _ F.state _ (L,V,s) (L,V',(stmtExp y (Var x) s')).
+Proof.
+  intros. 
+  eapply sim_expansion_closed. 
+  Focus 2. eapply star_refl.
+  Focus 2. eapply S_star. econstructor. simpl. reflexivity. eapply star_refl.
+  rewrite H.
+  eapply sim_eta. 
+  intros. lud. 
+  rewrite H0; eauto.
+  rewrite <- H0; eauto. eapply simLeq_refl.
+Qed.
+*)
+Unset Printing Records. 
+
+
+(*
+Inductive simL : F.labenv -> F.labenv -> Prop :=
+  | simLnil : simL nil nil
+  | simLcons L L' E E' Z Z' s s'
+    : (forall VL, 
+         sim (F.blockI E Z s::L, E[Z <-- VL], s) 
+             (F.blockI E' Z' s'::L', E'[Z' <-- VL], s'))
+      -> length Z = length Z'
+      -> simL L L'
+      -> simL (F.blockI E Z s::L) (F.blockI E' Z' s'::L').
+
+Lemma simL_refl L : simL L L.
+Proof.
+  induction L; eauto using simL.
+  destruct a. econstructor; intros; eauto. eapply sim_refl.
+Qed.
+
+Lemma simL_get L L' n blk blk'
+: simL L L'
+  -> get L n blk
+  -> get L' n blk'
+  -> (forall VL, 
+         sim (L, F.block_E blk[block_Z blk <-- VL], block_s blk) 
+             (L', F.block_E blk'[block_Z blk' <-- VL], block_s blk')) 
+     /\ length (block_Z blk) = length (block_Z blk').
+Proof.
+  intros. general induction H0. inv H1; inv H.
+  simpl. split; eauto. 
+Qed.
+*)    
+
+
+
+(*
+Lemma subst_lemma_sim L' s s' V E E' Z Z' L1 L2 t
+: simLeq L1 L2
+  -> (forall VL L L', simLeq L L' -> 
+        diverges F.step (L, E[Z <-- VL], s) 
+         -> diverges F.step (L', E'[Z' <-- VL], s'))
+  -> length Z = length Z'
+  -> length L1 = length L2
+  -> sim ((L' ++ F.blockI E Z s :: L1)%list, V, t)
+         ((L' ++ F.blockI E' Z' s' :: L2)%list, V, t).
+Proof.
+  revert_all; cofix; intros.
+  destruct t.
+  + exfalso; clear_all; admit.
+  + exfalso; clear_all; admit.
+  + destruct (get_subst _ _ _ Ldef) as [|[]].
+    - econstructor. econstructor. eapply len. eapply get_app; eauto. reflexivity.
+      pose proof (get_range H6). rewrite drop_length; eauto.
+      rewrite drop_length in H5. eapply subst_lemma_div; eauto. eauto.
+    - destruct H6; dcr; subst; simpl in *. 
+      econstructor. constructor. instantiate (1:= F.blockI E' Z' s').
+      simpl. eauto. congruence. simpl. rewrite H8. eapply get_length_app.
+      reflexivity. simpl. rewrite H8. rewrite drop_length_eq.
+      eapply (subst_lemma_div nil); eauto. simpl.
+      rewrite H8 in H5. rewrite drop_length_eq in H5.
+      unfold updE. eapply H0. Focus 2. unfold updE in H5. eapply H5.
+      eapply simLeq_refl. 
+      edestruct get_length_eq; try eassumption.
+      econstructor. econstructor. Focus 2. 
+      rewrite cons_app. rewrite app_assoc.
+      eapply get_app_right; eauto. simpl.
+      repeat rewrite app_length; simpl. omega.
+      Focus 2. 
+      reflexivity. Focus 2. simpl. rewrite drop_length_gr; eauto.
+      pose proof (H _ _ _ H7 H6).
+      unfold updE. unfold updE in H5.
+      rewrite drop_length_gr in H5.
+      refine (sim_codiverge (H9 _) H5). eassumption. 
+      exfalso; clear_all; admit.
+  + exfalso; clear_all; admit.
+  + econstructor. econstructor.
+    rewrite cons_app. rewrite app_assoc.
+    eapply (subst_lemma_div (F.blockI V Z0 s0::nil ++ L')%list); eauto.
+Qed.
+
+  + eapply simS; try eapply plusO.
+    econstructor; eauto.
+    econstructor; eauto.
+    eapply (subst_lemma_sim (F.blockI V Z0 t1::L')); eauto.
+Qed.
+*)
+*)
+
+(* 
+*** Local Variables: ***
+*** coq-load-path: (("." "Lvc")) ***
+*** End: ***
+*)
